outline of the PRF assumption for CHACHA20_POLY1305; still have to rewire AEAD to use it.

examples/low-level/crypto/Crypto.Symmetric.Chacha20.PRF.fst
@@ -22,81 +22,33 @@ module HH = FStar.HyperHeap
 module HS = FStar.HyperStack
 
 module MAC = Crypto.Symmetric.Poly1305.MAC
-module Block = Crypto.Symmetric.Chacha20
+module Chacha = Crypto.Symmetric.Chacha20
 
+let u8  = UInt8.t
+let u32 = UInt32.t
 let u64 = UInt64.t
+
+type domain = { nonce:u64; ctr:u32 } // could use lbytes 12 instead
 
 let blockLen = 64ul
 let block = b:bytes {Buffer.length b = v blockLen}
 
+type lbytes (l:uint32) = b:bytes {Buffer.length b = v l}
 
 // for now a bit too specific; 
 // we should be parametric in i for the size of blocks, for conditional idealization,...
 
 // the range of our PRF, after idealization and `reverse inlining`.
 
-type domain = { nonce:u64; ctr:u32 } // could use lbytes 12 instead
-
 type range (i:id) (x:domain) = if x.ctr = 0ul then MAC.state i nonce else block 
 type entry (i:id) = Entry: x:domain -> range i x -> entry i
 
 // the PRF instance, including the key and memoization table
 // TODO separate on rw, with multiple readers? 
-type state (i:id) = | State: 
-  rgn:i:id -> 
-  key:u32 -> 
-  log:rref rgn (Seq.seq (entry i)) -> state i // should be maybe_mrref; for later. 
-
-val prf_xor_1: key -> nonce -> ctr:u32 { ctr <> 0ul } -> msg:block -> Tot block
-val prf_xor: t -> nonce -> ctr:u32 { ctr <> 0ul } -> msg:block -> Tot block
-
-let prf_xor t nonce ctr msg = memoize t (fun () -> prf_xor_1 t.key nonce ctr msg)
-
-// for clarity, we use separate functions for each use of the PRF
-// But we still use a single, ctr-dependent range in the table. 
-
-let prf_mac i t (x:domain {x.ctr = 0ul}) = 
-  if ideal then 
-    begin 
-      match lookup t.log with 
-      | Some mac -> mac 
-      | None     -> let mac = MAC.gen (i,nonce) t.rgn in 
-                   write_at_end t.log (Entry iv ctr mac);
-                   mac 
-    end
-  else
-    let block = create 0ul blockLen in 
-    Block.chacha20 block t.key iv ctr Block.constant blockLen;
-    coerce i t.rgn (sub block 0ul MAC.keyLen)
-    
-  memoize t.log (fun () -> 
-
-
-let prf_xor t iv ctr maybe_block = 
-  if ideal then 
-    memoize (fun nonce ctr maybe_block -> 
-      if x.ctr = 0ul 
-      then 
-      else random blockLen)
-  else
-    let block = create 0ul blockLen in 
-    Block.chacha20 block t.key iv ctr Block.constant blockLen; //TODO truncate last block
-    if ctr = 0ul then 
-      coerce i region (sub block 0ul MAC.keyLen)
-    else
-      xor_bytes_inplace cipher plain len
-
-
- | MAC:  nonce:u64           -> block:block -> entry i
- | Mask: nonce:u64 -> ctr:u32 -> block:block -> entry i
-
-let log_ref (r:rid) (i:id) = log_t r (entry i)
-
-noeq type state (i:id) =
-  | State: rid: HH.rid
-         -> key: lbytes 32
-         -> log: log_ref i
-	 -> state i
+type state (i:id) = 
+  | State: rgn: HH.rid ->
+           key:u32 -> 
+           log:rref rgn (Seq.seq (entry i)) -> state i // should be maybe_mrref; for later. 
 
 assume val random: nat -> ST (seq u8)
   (requires (fun m -> True))
@@ -114,5 +66,84 @@ let gen i =
   let key = random 32 in
   let log = alloc_mref_seq Seq.createEmpty in
   State key log
+
+
+// generates a PRF block and copies its len first bytes to output
+let getBlock i t x len output = 
+  Chacha.chacha20 output t.key x.iv x.ctr Chacha.constant len;
+
+
+// We encapsulate the 3 usages of the PRF in specific functions.
+// But we still use a single, ctr-dependent range in the table. 
+//
+// For xor-based encryption, 
+// the ideal variant records both the plaintext and the ciphertext
+// whereas the real PRF output is their xor.
+
+// the first block (ctr=0) is used to generate a single-use MAC
+val prf_mac: i:id -> t:state i -> x:domain -> ST MAC.state (i,x.nonce)
+  (requires (fun h0 -> x.ctr = 0ul))
+  (ensures 
+    // we guarantee the stateful post of MAC.create when x is not in the table. 
+    // in all cases, we return the state in the table
+  )
+  
+// generates a fresh block for x and XORs it with plaintext
+val prf_enxor: i:id -> t:state i -> x:domain -> l:uint32 -> plain:lbytes l -> cipher:lbytes l -> STL unit 
+  (requires (fun h0 -> 
+     x.ctr <> 0ul /\ live h0 plain /\ live h0 cipher /\
+     is_None(lookupT h0 t.log x) 
+     ))
+  (ensures (fun h0 _ h1 -> 
+     modifies_1 cipher h0 h1 /\
+     match lookupT h0 t.log x with 
+     | Some (p,c) -> sel_word h1 plain == p /\ sel_word h1 cipher = c
+     | None -> False 
+     ))
+
+// reuse the same block for x and XORs it with ciphertext
+val prf_dexor: i:id -> t:state i -> x:domain -> l:uint32 -> plain:lbytes l -> cipher:lbytes l -> STL unit 
+  (requires (fun h0 -> 
+     x.ctr <> 0ul /\ live h0 plain /\ live h0 cipher /\
+     match lookupT h0 t.log x with 
+     | None -> False
+     | Some (p,c) -> sel_word h0 cipher == c
+     ))
+  (ensures (fun h0 _ h1 -> 
+     modifies_1 plain h0 h1 /\
+     match lookupT h0 t.log with 
+     | Some (p,c) -> sel_word h1 plain == p
+     | None -> False 
+     ))
+
+let prf_mac i t x = 
+  if ideal then (
+    match lookup t.log x with 
+    | Some mac -> mac 
+    | None     -> let mac = MAC.gen (i,nonce) t.rgn in 
+                 append t.log (Entry x mac);
+                 mac )
+  else (
+    let keyBytes = create 0uy keyLen in 
+    getBlock t x keyLen keyBytes;
+    coerce i t.rgn keyBytes )
+
+let prf_enxor i t x l output input = 
+  if ideal then (
+    let c = random_seq l in  
+    // store c into cipher 
+    append t.log (Entry x (input,output)))
+  else (
+    getBlock t x l output;
+    xor_bytes_inplace output input l ) 
+
+let prf_dexor i t x l output input = 
+  if ideal then ( 
+    match lookup t.log x with 
+    | Some (p,c) -> copy p to output )
+  else (
+    getBlock t x l output; 
+    xor_bytes_inplace output input l )
+
 
 
